Noperthedron/ComputationalStep.lean
@@ -1,11 +1,23 @@
+import Noperthedron.Checker.RowZero
 import Noperthedron.PoseInterval
 import Noperthedron.SolutionTable
+import Noperthedron.SolutionTable.Parse
 import Noperthedron.Vertices.Exact
 
 namespace Noperthedron
 
---def csv : String := include_str "../../noperthedron-verification-py/data/solution_tree.csv"
-
-theorem exists_solution_table : ∃ (tab : Solution.ValidTable), True
-     := by
-  sorry -- TODO(hard)
+theorem exists_solution_table : ∃ (tab : Solution.ValidTable), True := by
+  sorry
+  /-
+  let solution_csv : String :=
+    include_str "../../noperthedron-verification-py/data/solution_tree.csv"
+  let tab := match Solution.parseSolutionTable solution_csv with
+             | .ok s => s
+             | .error _ => #[]
+  have hnonempty : 0 < tab.size := by native_decide
+  have hrowzero : tab[0].interval = Solution.rowZero.interval := by native_decide
+  have hvalid : tab.RowsValid := by native_decide
+  refine ⟨⟨tab, hvalid, hnonempty, ?_⟩, ⟨⟩⟩
+  rw [hrowzero]
+  exact Solution.rowZero_contains_tightInterval
+  -/
